common/GlobalenvsC.v
@@ -1,0 +1,350 @@
+Require Recdef.
+Require Import Zwf.
+Require Import Axioms CoqlibC Errors MapsC AST Linking.
+Require Import Integers Floats Values Memory.
+Require Import sflib.
+
+Require Export Globalenvs.
+
+Require Import sflib.
+From Paco Require Import paco.
+
+Notation "s #1" := (fst s) (at level 9, format "s '#1'") : pair_scope.
+Notation "s #2" := (snd s) (at level 9, format "s '#2'") : pair_scope.
+
+Local Open Scope pair_scope.
+
+Set Implicit Arguments.
+
+
+
+
+Section MAP.
+
+  Variable F1 V1 F2 V2: Type.
+
+  Program Definition Genv_map_defs (ge0: Genv.t F1 V1)
+          (f: globdef F1 V1 -> option (globdef F2 V2)): Genv.t F2 V2 :=
+  {|
+    Genv.genv_public := ge0.(Genv.genv_public);
+    Genv.genv_symb := ge0.(Genv.genv_symb);
+    Genv.genv_defs := ge0.(Genv.genv_defs).(PTree_filter_map (fun _ => f));
+    Genv.genv_next := ge0.(Genv.genv_next);
+  |}
+  .
+  Next Obligation. eapply Genv.genv_symb_range; eauto. Qed.
+  Next Obligation. rewrite PTree_filter_map_spec in H. u. des_ifs. eapply Genv.genv_defs_range; eauto. Qed.
+  Next Obligation. eapply Genv.genv_vars_inj; eauto. Qed.
+
+  (* Note: genv_defs will have spurious data, but this is actually Compcert's interpretation. *)
+  Program Definition Genv_filter_symb (ge0: Genv.t F1 V1)
+          (f: ident -> bool): Genv.t F1 V1 :=
+  {|
+    Genv.genv_public := ge0.(Genv.genv_public);
+    Genv.genv_symb := ge0.(Genv.genv_symb).(PTree_filter_key f);
+    Genv.genv_defs := ge0.(Genv.genv_defs);
+    Genv.genv_next := ge0.(Genv.genv_next);
+  |}
+  .
+  Next Obligation. rewrite PTree_filter_key_spec in *. des_ifs. eapply Genv.genv_symb_range; eauto. Qed.
+  Next Obligation. eapply Genv.genv_defs_range; eauto. Qed.
+  Next Obligation. rewrite PTree_filter_key_spec in *. des_ifs. eapply Genv.genv_vars_inj; eauto. Qed.
+
+
+End MAP.
+
+
+
+(* Below may not be needed *)
+Section MATCH_PROGRAMS_BACKWARD.
+
+Context {C F1 V1 F2 V2: Type} {LC: Linker C} {LF: Linker F1} {LV: Linker V1}.
+(* Variable transf_fundef: C -> F1 -> option F2. *)
+(* Let match_fundef: C -> F1 -> F2 -> Prop := fun c f tf => transf_fundef c f = Some tf. *)
+Variable match_fundef: C -> F1 -> F2 -> Prop.
+Variable match_varinfo: V1 -> V2 -> Prop.
+Variable ctx: C.
+Variable p: program F1 V1.
+Variable tp: program F2 V2.
+Hypothesis progmatch: match_program_gen match_fundef match_varinfo ctx p tp.
+
+Theorem find_def_match_backward:
+  forall b tg,
+  Genv.find_def (Genv.globalenv tp) b = Some tg ->
+  exists g,
+  Genv.find_def (Genv.globalenv p) b = Some g /\ match_globdef match_fundef match_varinfo ctx g tg.
+Proof.
+  intros. generalize (Genv.find_def_match_2 progmatch b). rewrite H; intros R; inv R.
+  exists x; auto.
+Qed.
+
+Theorem find_funct_ptr_match_backward:
+  forall b tf,
+  Genv.find_funct_ptr (Genv.globalenv tp) b = Some tf ->
+  exists cunit f,
+  Genv.find_funct_ptr (Genv.globalenv p) b = Some f /\ match_fundef cunit f tf /\ linkorder cunit ctx.
+Proof.
+  intros. rewrite Genv.find_funct_ptr_iff in *. apply find_def_match_backward in H.
+  destruct H as (tg & P & Q). inv Q.
+  exists ctx', f1; intuition auto. apply Genv.find_funct_ptr_iff; auto.
+Qed.
+
+Theorem find_funct_match_backward:
+  forall v tf,
+  Genv.find_funct (Genv.globalenv tp) v = Some tf ->
+  exists cunit f,
+  Genv.find_funct (Genv.globalenv p) v = Some f /\ match_fundef cunit f tf /\ linkorder cunit ctx.
+Proof.
+  intros. exploit Genv.find_funct_inv; eauto. intros [b EQ]. subst v.
+  rewrite Genv.find_funct_find_funct_ptr in H.
+  rewrite Genv.find_funct_find_funct_ptr.
+  apply find_funct_ptr_match_backward. auto.
+Qed.
+
+Theorem find_var_info_match_backward:
+  forall b tv,
+  Genv.find_var_info (Genv.globalenv tp) b = Some tv ->
+  exists v,
+  Genv.find_var_info (Genv.globalenv p) b = Some v /\ match_globvar match_varinfo v tv.
+Proof.
+  intros. rewrite Genv.find_var_info_iff in *. apply find_def_match_backward in H.
+  destruct H as (tg & P & Q). inv Q.
+  exists v1; split; auto. apply Genv.find_var_info_iff; auto.
+Qed.
+
+Lemma store_init_data_list_match_backward:
+  forall idl m b ofs m',
+  Genv.store_init_data_list (Genv.globalenv tp) m b ofs idl = Some m' ->
+  Genv.store_init_data_list (Genv.globalenv p) m b ofs idl = Some m'.
+Proof.
+  induction idl; simpl; intros.
+- auto.
+- destruct (Genv.store_init_data (Genv.globalenv tp) m b ofs a) as [m1|] eqn:S; try discriminate.
+  assert (X: Genv.store_init_data (Genv.globalenv p) m b ofs a = Some m1).
+  { destruct a; auto. simpl; rewrite <- (Genv.find_symbol_match progmatch); auto. }
+  rewrite X. auto.
+Qed.
+
+Lemma alloc_globals_match_backward:
+  forall gl1 gl2, list_forall2 (match_ident_globdef match_fundef match_varinfo ctx) gl1 gl2 ->
+  forall m m',
+  Genv.alloc_globals (Genv.globalenv tp) m gl2 = Some m' ->
+  Genv.alloc_globals (Genv.globalenv p) m gl1 = Some m'.
+Proof.
+  induction 1; simpl; intros.
+- auto.
+- destruct (Genv.alloc_global (Genv.globalenv tp) m b1) as [m1|] eqn:?; try discriminate.
+  assert (X: Genv.alloc_global (Genv.globalenv p) m a1 = Some m1).
+  { destruct a1 as [id1 g1]; destruct b1 as [id2 g2]; destruct H; simpl in *.
+    subst id2. inv H2.
+  - auto.
+  - inv H; simpl in *.
+    set (sz := init_data_list_size init) in *.
+    destruct (Mem.alloc m 0 sz) as [m2 b] eqn:?.
+    destruct (store_zeros m2 b 0 sz) as [m3|] eqn:?; try discriminate.
+    destruct (Genv.store_init_data_list (Genv.globalenv tp) m3 b 0 init) as [m4|] eqn:?; try discriminate.
+    erewrite store_init_data_list_match_backward; eauto.
+  }
+  rewrite X; eauto.
+Qed.
+
+Theorem init_mem_match_backward:
+  forall m, Genv.init_mem tp = Some m -> Genv.init_mem p = Some m.
+Proof.
+  unfold Genv.init_mem; intros.
+  eapply alloc_globals_match_backward; eauto. apply progmatch.
+Qed.
+
+End MATCH_PROGRAMS_BACKWARD.
+
+Program Instance Senv_eq_equiv: RelationClasses.Equivalence Senv.equiv.
+Next Obligation.
+  ii.
+  econs; eauto.
+Qed.
+Next Obligation.
+  ii.
+  inv H. des.
+  econs; eauto.
+Qed.
+Next Obligation.
+  ii.
+  inv H. inv H0. des.
+  econs; eauto.
+  i. erewrite <- H1; eauto.
+Qed.
+
+
+
+Inductive good_genv {F V} (ge: Genv.t F V): Prop :=
+| good_genv_intro
+    (FIND_SYMBOL: forall id b,
+        Genv.find_symbol ge id = Some b -> (exists g, Genv.find_def ge b = Some g))
+    (FIND_DEF: forall b g,
+        Genv.find_def ge b = Some g -> (exists id, Genv.find_symbol ge id = Some b))
+.
+
+Inductive genv_precise {F V} (ge: Genv.t F V) (p: program F V): Prop :=
+| genv_compat_intro
+    (FIND_MAP: forall id g,
+        p.(prog_defmap) ! id = Some g ->
+        (exists b, Genv.find_symbol ge id = Some b /\ Genv.find_def ge b = Some g))
+    (FIND_MAP_INV: forall id b g,
+        (Genv.find_symbol ge id = Some b /\ Genv.find_def ge b = Some g) ->
+        p.(prog_defmap) ! id = Some g)
+.
+
+
+
+(* Module PLAYGROUND0. *)
+
+(* Section INJECT. *)
+
+(*   Variables F1 V1 F2 V2: Type. *)
+(*   Variable ge1: Genv.t F1 V1. *)
+(*   Variable ge2: Genv.t F2 V2. *)
+
+(*   (* Record meminj_preserves_globals (f: meminj) : Prop := { *) *)
+(*   (*   symbols_inject_1: forall id b b' delta, *) *)
+(*   (*     f b = Some(b', delta) -> Genv.find_symbol ge id = Some b -> *) *)
+(*   (*     delta = 0 /\ Genv.find_symbol tge id = Some b'; *) *)
+(*   (*   symbols_inject_2: forall id b, *) *)
+(*   (*     kept id -> Genv.find_symbol ge id = Some b -> *) *)
+(*   (*     exists b', Genv.find_symbol tge id = Some b' /\ f b = Some(b', 0); *) *)
+(*   (*   symbols_inject_3: forall id b', *) *)
+(*   (*     Genv.find_symbol tge id = Some b' -> *) *)
+(*   (*     exists b, Genv.find_symbol ge id = Some b /\ f b = Some(b', 0); *) *)
+(*   (*   defs_inject: forall b b' delta gd, *) *)
+(*   (*     f b = Some(b', delta) -> Genv.find_def ge b = Some gd -> *) *)
+(*   (*     Genv.find_def tge b' = Some gd /\ delta = 0 /\ *) *)
+(*   (*     (forall id, ref_def gd id -> kept id); *) *)
+(*   (*   defs_rev_inject: forall b b' delta gd, *) *)
+(*   (*     f b = Some(b', delta) -> Genv.find_def tge b' = Some gd -> *) *)
+(*   (*     Genv.find_def ge b = Some gd /\ delta = 0 *) *)
+(*   (* }. *) *)
+
+(*   (* Definition init_meminj : meminj := *) *)
+(*   (*   fun b => *) *)
+(*   (*     match Genv.invert_symbol ge b with *) *)
+(*   (*     | Some id => *) *)
+(*   (*       match Genv.find_symbol tge id with *) *)
+(*   (*       | Some b' => Some (b', 0) *) *)
+(*   (*       | None => None *) *)
+(*   (*       end *) *)
+(*   (*     | None => None *) *)
+(*   (*     end. *) *)
+
+
+(*   Record symbols_inject (f: meminj): Prop := { *)
+(*     public: (forall id, Senv.public_symbol ge2 id = Senv.public_symbol ge1 id); *)
+(*     inject: (forall id b1 b2 delta, *)
+(*                  f b1 = Some(b2, delta) -> Senv.find_symbol ge1 id = Some b1 -> *)
+(*                  delta = 0 /\ Senv.find_symbol ge2 id = Some b2); *)
+(*     public_find: (forall id b1, *)
+(*                      Senv.public_symbol ge1 id = true -> Senv.find_symbol ge1 id = Some b1 -> *)
+(*                      exists b2, f b1 = Some(b2, 0) /\ Senv.find_symbol ge2 id = Some b2); *)
+(*   } *)
+(*   . *)
+
+(*   (* Definition symbols_inject (f: meminj): Prop := *) *)
+(*   (*   (forall id, Senv.public_symbol ge2 id = Senv.public_symbol ge1 id) *) *)
+(*   (*   /\ (forall id b1 b2 delta, *) *)
+(*   (*          f b1 = Some(b2, delta) -> Senv.find_symbol ge1 id = Some b1 -> *) *)
+(*   (*          delta = 0 /\ Senv.find_symbol ge2 id = Some b2) *) *)
+(*   (*   /\ (forall id b1, *) *)
+(*   (*          Senv.public_symbol ge1 id = true -> Senv.find_symbol ge1 id = Some b1 -> *) *)
+(*   (*          exists b2, f b1 = Some(b2, 0) /\ Senv.find_symbol ge2 id = Some b2) *) *)
+(*   (*   /\ (forall b1 b2 delta, *) *)
+(*   (*          f b1 = Some(b2, delta) -> *) *)
+(*   (*          Senv.block_is_volatile ge2 b2 = Senv.block_is_volatile ge1 b1). *) *)
+
+(*   Inductive match_globalenvs (f: meminj) (bound: block): Prop := *)
+(*   | mk_match_globalenvs *)
+(*       (DOMAIN: forall b, Plt b bound -> f b = Some(b, 0)) *)
+(*       (IMAGE: forall b1 b2 delta, f b1 = Some(b2, delta) -> Plt b2 bound -> b1 = b2) *)
+(*       (SYMBOLS: forall id b, Genv.find_symbol ge1 id = Some b -> Plt b bound) *)
+(*       (FUNCTIONS: forall b fd, Genv.find_funct_ptr ge1 b = Some fd -> Plt b bound) *)
+(*       (VARINFOS: forall b gv, Genv.find_var_info ge1 b = Some gv -> Plt b bound) *)
+(*   . *)
+
+(*   Lemma ABC *)
+(*         f *)
+(*         (GOODSRC: good_genv ge1) *)
+(*         (GOODTGT: good_genv ge2) *)
+(*         (RECIPE: recipe_consistent f recipe_normal) *)
+(*         (INJ: symbols_inject f) *)
+(*         (FLAT: f = (Mem.flat_inj ge1.(Genv.genv_next))) *)
+(*     : *)
+(*       match_globalenvs f ge1.(Genv.genv_next) *)
+(*   . *)
+(*   Proof. *)
+(*     (* unfold symbols_inject in *. des. *) *)
+(*     unfold Mem.flat_inj in *. des_ifs; ss. *)
+(*     inv RECIPE. *)
+(*     econs; i; des_ifs; ss. *)
+(*     - destruct (Genv.public_symbol ge1 id) eqn:T. *)
+(*       + hexploit public_find; try eassumption. *)
+(*         i; des. unfold Mem.flat_inj in *. des_ifs. *)
+(*       + exploit PRIVATES; eauto. i; des. des_ifs. *)
+(*     - unfold Genv.find_funct_ptr in *. *)
+(*       des_ifs. *)
+(*       inv GOODSRC. *)
+(*       exploit FIND_DEF; eauto. i; des. *)
+(*       destruct (Genv.public_symbol ge1 id) eqn:T. *)
+(*       + exploit public_find; try eassumption. *)
+(*         i; des. unfold Mem.flat_inj in *. des_ifs. *)
+(*       + exploit PRIVATES; eauto. i; des. des_ifs. *)
+(*     - unfold Genv.find_var_info in *. *)
+(*       des_ifs. *)
+(*       inv GOODSRC. *)
+(*       exploit FIND_DEF; eauto. *)
+(*       i; des. *)
+(*       destruct (Genv.public_symbol ge1 id) eqn:T. *)
+(*       + exploit public_find; try eassumption. *)
+(*         i; des. unfold Mem.flat_inj in *. des_ifs. *)
+(*       + exploit PRIVATES; eauto. i; des. des_ifs. *)
+(*   Qed. *)
+
+(*   Lemma ABCD *)
+(*         f *)
+(*         (GOODSRC: good_genv ge1) *)
+(*         (GOODTGT: good_genv ge2) *)
+(*         (RECIPE: recipe_consistent f recipe_normal) *)
+(*         (INJ: symbols_inject f) *)
+(*     : *)
+(*       match_globalenvs f ge1.(Genv.genv_next) *)
+(*   . *)
+(*   Proof. *)
+(*     inv RECIPE. *)
+(*     econs; i; des_ifs; ss. *)
+(*   Abort. *)
+
+(* End INJECT. *)
+
+(* End PLAYGROUND0. *)
+
+
+(* Module PLAYGROUND1. *)
+
+(* Section INJECT. *)
+
+(*   Variables F1 V1 F2 V2: Type. *)
+(*   Variable prog1: program F1 V1. *)
+(*   Variable prog2: program F2 V2. *)
+(*   Variable ge1: Genv.t F1 V1. *)
+(*   Variable ge2: Genv.t F2 V2. *)
+(*   Hypothesis COMPAT1: genv_compat ge1 (prog_defmap prog1). *)
+(*   Hypothesis COMPAT2: genv_compat ge2 (prog_defmap prog2). *)
+(*   Hypothesis GOOD1: good_genv ge1. *)
+(*   Hypothesis GOOD2: good_genv ge2. *)
+(*   Variable match_gdef: ident * globdef F1 V1 -> ident * globdef F2 V2 -> Prop. *)
+(*   (* (match_ident_globdef match_fundef match_varinfo ctx) *) *)
+(*   Hypothesis MATCH: list_forall2 match_gdef (prog_defs prog1) (prog_defs prog2). *)
+
+(*   Hypothesis SYMBINJ: symbols_inject ge1 ge2. *)
+
+(* End INJECT. *)
+
+(* End PLAYGROUND1. *)
+
+
